examples/dsls/core/FStar.Meta.Tc.Builtins.fsti
@@ -1,8 +1,38 @@
 module FStar.Meta.Tc.Builtins
 
-open FStar.Reflection.Types
+open FStar.Reflection
 open FStar.Meta.Tc.Effect
 
-val valid_prop (en:env) (t:typ) : Type0
+open FStar.Reflection.Helpers
+open FStar.Reflection.Subst
 
-val check_prop_validity (en:env) (t:typ) : MetaTcT (valid_prop en t)
+val valid_prop_token (en:env) (t:typ) : Type0
+val subtyping_token (en:env) (t1 t2:typ) : Type0
+
+///
+/// Should these return option or raise exceptions?
+/// 
+
+val check_prop_validity (en:env) (t:typ) : MetaTcT (valid_prop_token en t)
+val check_subtyping (en:env) (t1 t2:typ) : MetaTcT (option (subtyping_token en t1 t2))
+
+val subtyping_token_renaming (g:env)
+                             (bs0:bindings)
+                             (bs1:bindings)
+                             (x:var { None? (lookup_bvar (extend_env_l g (bs1@bs0)) x) })
+                             (y:var { None? (lookup_bvar (extend_env_l g (bs1@bs0)) y) })
+                             (t:term)
+                             (t0 t1:term)
+                             (d:subtyping_token (extend_env_l g (bs1@(x,t)::bs0)) t0 t1)
+  : subtyping_token (extend_env_l g (rename_bindings bs1 x y@(y,t)::bs0))
+                    (rename t0 x y)
+                    (rename t1 x y)
+
+val subtyping_token_weakening (g:env)
+                              (bs0:bindings)
+                              (bs1:bindings)
+                              (x:var { None? (lookup_bvar (extend_env_l g (bs1@bs0)) x) })
+                              (t:term)
+                              (t0 t1:term)
+                             (d:subtyping_token (extend_env_l g (bs1@bs0)) t0 t1)
+  : subtyping_token (extend_env_l g (bs1@(x,t)::bs0)) t0 t1
