examples/dsls/core/FStar.Reflection.Helpers.fsti
@@ -1,0 +1,122 @@
+module FStar.Reflection.Helpers
+
+open FStar.Reflection
+module R = FStar.Reflection
+
+//
+// Should move to ulib
+//
+
+val inspect_pack (t:R.term_view)
+  : Lemma (ensures R.(inspect_ln (pack_ln t) == t))
+          [SMTPat R.(inspect_ln (pack_ln t))]
+
+val pack_inspect (t:R.term)
+  : Lemma (ensures R.(pack_ln (inspect_ln t) == t))
+          [SMTPat R.(pack_ln (inspect_ln t))]
+
+val inspect_pack_bv (t:R.bv_view)
+  : Lemma (ensures R.(inspect_bv (pack_bv t) == t))
+          [SMTPat R.(inspect_bv (pack_bv t))]
+
+val pack_inspect_bv (t:R.bv)
+  : Lemma (ensures R.(pack_bv (inspect_bv t) == t))
+          [SMTPat R.(pack_bv (inspect_bv t))]
+
+val inspect_pack_binder (b:_) (q:_) (a:_)
+  : Lemma (ensures R.(R.inspect_binder (R.pack_binder b q a) == (b, (q, a))))
+          [SMTPat R.(inspect_binder (pack_binder b q a))]
+
+val pack_inspect_binder (t:R.binder)
+  : Lemma (ensures (let b, (q, a) = R.inspect_binder t in
+                    R.(pack_binder b q a == t)))
+
+val pack_inspect_comp (t:R.comp)
+  : Lemma (ensures (R.pack_comp (R.inspect_comp t) == t))
+          [SMTPat (R.pack_comp (R.inspect_comp t))]
+
+val inspect_pack_comp (t:R.comp_view)
+  : Lemma (ensures (R.inspect_comp (R.pack_comp t) == t))
+          [SMTPat (R.inspect_comp (R.pack_comp t))]
+
+val lookup_bvar (e:env) (x:int) : option term
+
+val lookup_fvar (e:env) (x:fv) : option term
+
+val extend_env (e:env) (x:var) (ty:term) : env
+
+val lookup_bvar_extend_env (g:env) (x y:var) (ty:term)
+  : Lemma 
+    (ensures (
+           if x = y
+           then lookup_bvar (extend_env g x ty) y == Some ty
+           else lookup_bvar (extend_env g x ty) y == lookup_bvar g y))
+    [SMTPat (lookup_bvar (extend_env g x ty) y)]
+
+val lookup_fvar_extend_env (g:env) (x:fv) (y:var) (ty:term)
+  : Lemma 
+    (ensures lookup_fvar (extend_env g y ty) x == lookup_fvar g x)
+    [SMTPat (lookup_fvar (extend_env g y ty) x)]
+
+let as_binder (x:var) (ty:term)
+  : binder 
+  = pack_binder
+      (pack_bv ({bv_ppname="";
+                 bv_index=x;
+                 bv_sort=ty}))
+      Q_Explicit
+      []
+
+let bv_index (x:bv) : int = (inspect_bv x).bv_index
+
+let binder_sort (b:binder) =
+  let bv, _ = inspect_binder b in 
+  (inspect_bv bv).bv_sort
+
+let binder_sort_lemma (x:var) (ty:term)
+  : Lemma (binder_sort (as_binder x ty) == ty)
+          [SMTPat (binder_sort (as_binder x ty))]
+  = ()
+
+type guard = option typ
+
+let bv_as_binder bv = pack_binder bv Q_Explicit []
+
+let make_bv (n:nat) (t:term) = { bv_ppname = "_"; bv_index = n; bv_sort = t}
+let var_as_bv (v:var) = pack_bv (make_bv v (pack_ln Tv_Unknown))
+let var_as_term (v:var) = pack_ln (Tv_Var (var_as_bv v))
+
+let bv_index_of_make_bv (n:nat) (t:term)
+  : Lemma (ensures bv_index (pack_bv (make_bv n t)) == n)
+          [SMTPat (bv_index (pack_bv (make_bv n t)))]
+  = ()
+
+let constant_as_term (v:vconst) = pack_ln (Tv_Const v)
+let unit_exp = constant_as_term C_Unit
+let unit_fv = pack_fv unit_lid
+let unit_ty = pack_ln (Tv_FVar unit_fv)
+let bool_fv = pack_fv bool_lid
+let bool_ty = pack_ln (Tv_FVar bool_fv)
+
+let mk_total u t = pack_comp (C_Total t u [])
+let tm_type u = pack_ln (Tv_Type u)
+
+let true_bool = pack_ln (Tv_Const C_True)
+let false_bool = pack_ln (Tv_Const C_False)
+let eq2 (t v0 v1:term) 
+  : term 
+  = let eq2 = pack_ln (Tv_FVar (pack_fv eq2_qn)) in
+    let h = pack_ln (Tv_App eq2 (t, Q_Implicit)) in
+    let h1 = pack_ln (Tv_App h (v0, Q_Explicit)) in
+    let h2 = pack_ln (Tv_App h1 (v1, Q_Explicit)) in    
+    h2
+
+val mk_conj (t1 t2:typ) : typ
+
+let bindings = list (var & term)
+
+let rec extend_env_l (g:env) (bs:bindings) 
+  : env
+  = match bs with
+    | [] -> g
+    | (x,t)::bs -> extend_env (extend_env_l g bs) x t
