examples/dsls/core/FStar.Reflection.Typing.fsti
@@ -1,0 +1,192 @@
+module FStar.Reflection.Typing
+
+open FStar.Reflection
+open FStar.Reflection.Helpers
+open FStar.Reflection.Subst
+
+open FStar.Meta.Tc.Builtins
+
+module R = FStar.Reflection
+
+let ( ++ ) : guard -> guard -> guard = fun g1 g2 ->
+  match g1, g2 with
+  | None, _ -> g2
+  | _, None -> g1
+  | Some g1, Some g2 -> Some (mk_conj g1 g2)
+
+[@@ erasable]
+noeq
+type typing_const : vconst -> typ -> Type =
+  | CT_Unit: typing_const C_Unit unit_ty
+  | CT_True: typing_const C_True bool_ty
+  | CT_False: typing_const C_False bool_ty
+
+
+//
+// TODO: should comp have universes?
+//
+
+[@@ erasable; no_auto_projectors]
+noeq
+type typing : env -> term -> comp -> guard -> Type =
+  | T_Var : 
+     g:env ->
+     x:bv { Some? (lookup_bvar g (bv_index x)) } ->
+     typing g (pack_ln (Tv_Var x))
+              (mk_total u_unk (Some?.v (lookup_bvar g (bv_index x))))
+              None
+
+  | T_FVar :
+     g:env ->
+     x:fv { Some? (lookup_fvar g x) } -> 
+     typing g (pack_ln (Tv_FVar x))
+              (mk_total u_unk (Some?.v (lookup_fvar g x)))
+              None
+  | T_Const:
+     g:env ->
+     v:vconst ->
+     t:term ->
+     typing_const v t ->
+     typing g (constant_as_term v) (mk_total u_unk t) None
+                        
+  | T_Abs :
+     g:env ->
+     x:var { None? (lookup_bvar g x) } ->
+     t:term ->
+     u_t:universe ->
+     g_t:guard ->
+     e:term ->
+     c:comp ->
+     g_e:guard ->
+     typing g t (mk_total u_unk (tm_type u_t)) g_t ->
+     typing (extend_env g x t) (open_term e x) c g_e ->
+     typing g (pack_ln (Tv_Abs (as_binder 0 t) e))
+              (mk_total u_unk (pack_ln (Tv_Arrow (as_binder 0 t) 
+                                       (close_comp c x))))
+              (g_t ++ close_guard g_e x)
+
+  | T_App :
+     g:env ->
+     e1:term ->
+     e2:term ->
+     x:binder ->
+     c:comp ->
+     g_e1:guard ->
+     g_e2:guard ->
+     typing g e1 (mk_total u_unk (pack_ln (Tv_Arrow x c))) g_e1 ->
+     typing g e2 (mk_total u_unk (binder_sort x)) g_e2 ->
+     typing g (pack_ln (Tv_App e1 (e2, Q_Explicit)))
+              (open_comp_with c e2)
+              (g_e1 ++ g_e2)
+
+  | T_Arrow:
+     g:env ->
+     x:var { None? (lookup_bvar g x) } ->
+     t:term ->
+     u_t:universe ->
+     g_t:guard ->
+     c:comp ->
+     u_c:universe ->
+     g_c:guard ->
+     typing g t (mk_total u_unk (tm_type u_t)) g_t ->
+     typing_comp (extend_env g x t) (open_comp c x) u_c g_c ->
+     typing g (pack_ln (Tv_Arrow (as_binder 0 t) c))
+              (mk_total u_unk (tm_type (pack_universe (Uv_Max [u_t; u_c]))))
+              (g_t ++ close_guard g_c x)
+
+  | T_Refine:
+     g:env ->
+     x:var { None? (lookup_bvar g x) } ->     
+     t:term ->
+     u_t:universe ->
+     g_t:guard ->
+     e:term ->
+     u_e:universe ->
+     g_e:guard ->
+     typing g t (mk_total u_unk (tm_type u_t)) g_t ->
+     typing (extend_env g x t) (open_term e x) (mk_total u_unk (tm_type u_e)) g_e ->
+     typing g (pack_ln (Tv_Refine (pack_bv (make_bv 0 t)) e))
+              (mk_total u_unk (tm_type u_t))
+              (g_t ++ close_guard g_e x)
+
+    //
+    // TODO: what about well-typedness of c2?
+    //
+
+  | T_Sub:
+     g:env ->
+     e:term ->
+     c1:comp ->
+     g_e:guard ->
+     c2:comp ->
+     g_sub:guard ->
+     typing g e c1 g_e ->
+     sub_comp g c1 c2 g_sub ->
+     typing g e c2 (g_e ++ g_sub)
+
+  | T_If: 
+     g:env ->
+     scrutinee:term ->
+     g_scrutinee:guard ->
+     then_:term ->
+     g_then:guard ->
+     else_:term ->
+     g_else:guard ->
+     c:comp ->
+     hyp:var { None? (lookup_bvar g hyp) } ->
+     typing g scrutinee (mk_total u_unk bool_ty) g_scrutinee ->
+     typing (extend_env g hyp (eq2 bool_ty scrutinee true_bool)) then_ c g_then ->
+     typing (extend_env g hyp (eq2 bool_ty scrutinee false_bool)) else_ c g_else ->
+     typing g (pack_ln (Tv_Match scrutinee None [(Pat_Constant C_True, then_); 
+                                                 (Pat_Constant C_False, else_)]))
+              c
+              (g_scrutinee ++ g_then ++ g_else)
+
+  | T_Match: 
+     g:env ->
+     scrutinee:term ->
+     i_ty:term ->
+     g_scrutinee:guard ->
+     branches:list branch ->
+     c:comp ->
+     g_branches:guard ->
+     typing g scrutinee (mk_total u_unk i_ty) g_scrutinee ->
+     branches_typing g scrutinee i_ty branches c g_branches ->
+     typing g (pack_ln (Tv_Match scrutinee None branches))
+              c
+              (g_scrutinee ++ g_branches)
+    
+and typing_comp : env -> comp -> universe -> guard -> Type =
+  | C_Total:
+     g:env ->
+     t:typ ->
+     u_t:universe ->
+     g_t:guard ->
+     typing g t (mk_total u_unk (tm_type u_t)) g_t ->
+     typing_comp g (mk_total u_unk t) u_t g_t
+
+and sub_typing : env -> term -> term -> guard -> Type0 =
+  | ST_Refl: 
+     g:env ->
+     t:term ->
+     sub_typing g t t None
+
+  | ST_Token: 
+     g:env ->
+     t1:term ->
+     t2:term ->      
+     subtyping_token g t1 t2 ->
+     sub_typing g t1 t2 None
+
+and sub_comp : env -> comp -> comp -> guard -> Type0 =
+  | SC_Total:
+     g:env ->
+     t1:typ ->
+     t2:typ ->
+     g_sub:guard ->
+     sub_typing g t1 t2 g_sub ->
+     sub_comp g (mk_total u_unk t1)
+                (mk_total u_unk t2)
+                g_sub
+
+and branches_typing : env -> term -> term -> list branch -> comp -> guard -> Type0 =
